if-else finished, 1 lemma left

WeirdLogic/Example1.lean
@@ -17,9 +17,8 @@ open ContextFreeGrammar
 namespace WeirdLogic
 
 /- L -> trm1 | trm 2 -/
-def trm0 : trm := [lang| xx := !y]
-def trm1 : trm := [lang| y := xx + 1]
-def trm2 : trm := [lang| y := xx + 2]
+def trm1 : trm := [lang| fun ⸨xk: Loc⸩ => let xx := !xk in let temp0 := xx + 1 in xk := temp0]
+def trm2 : trm := [lang| fun ⸨xr: Loc⸩ => let xx := !xr in let temp0 := xx + 2 in xr := temp0]
 def r1 : ContextFreeRule trm String :=
   {
     input := "L",
@@ -36,7 +35,7 @@ def cfg1 : ContextFreeGrammar trm :=
   {
     NT := String,
     initial := "L",
-    rules := Finset.mk {r1, r2} (by unfold r1 r2 trm1 trm2; simp)
+    rules := Finset.mk {r1, r2} (by unfold r1 r2 trm1 trm2 trm_funs; simp  )
   }
 
 def l1 : Language trm := cfg1.language
@@ -54,8 +53,11 @@ abbrev lang := List trm
 
 def cfg_expand : Set ( List (Symbol T N)) :=
   {
-    [Symbol.terminal trm0, Symbol.terminal trm1],[Symbol.terminal trm0, Symbol.terminal trm2]
+    [Symbol.terminal trm1],[Symbol.terminal trm2]
   }
+  -- {
+  --   [Symbol.terminal trm0, Symbol.terminal trm1],[Symbol.terminal trm0, Symbol.terminal trm2]
+  -- }
   -- {
   --   c | cfg1.Generates c
   -- }
@@ -81,13 +83,14 @@ def lang_list_index' : Set lang :=
   {l | (trm_to_symbol_list l) ∈ cfg_expand }
 
 def lang_index' : Set trm :=
+  -- {trm1, trm2}
   {squeeze_trm t | t ∈ lang_list_index'}
 
 def lang_index : Set (trm × payload ):=
   { (l,0) | l ∈ lang_index' }
 
 lemma lang_unfold :
-  lang_list_index' = {[trm0, trm1],[trm0, trm2]} := by
+  lang_list_index' = {[trm1],[trm2]} := by
   unfold lang_list_index' trm_to_symbol_list cfg_expand -- Generates Derives Produces expand_trm
   ext l
   simp
@@ -114,10 +117,29 @@ lemma lang_unfold :
   }
 
 lemma lang_index'_unfold :
-  lang_index' = {trm_seq trm0 trm1,trm_seq trm0 trm2} := by
+  lang_index' = {trm1,trm2} := by
   unfold lang_index' squeeze_trm
   rw [lang_unfold]
-  aesop
+  simp_all only [Set.mem_insert_iff, Set.mem_singleton_iff, exists_eq_or_imp, exists_eq_left]
+  ext x : 1
+  simp_all only [Set.mem_setOf_eq, Set.mem_insert_iff, Set.mem_singleton_iff]
+  apply Iff.intro
+  · intro a
+    cases a with
+    | inl h =>
+      subst h
+      simp_all only [true_or]
+    | inr h_1 =>
+      subst h_1
+      simp_all only [or_true]
+  · intro a
+    cases a with
+    | inl h =>
+      subst h
+      simp_all only [true_or]
+    | inr h_1 =>
+      subst h_1
+      simp_all only [or_true]
 
 def cfg1_left : ContextFreeGrammar trm :=
   {
@@ -156,9 +178,9 @@ abbrev default_payload : payload:= 0
 abbrev default_trm : trm := [lang|()]
 
 def lang_set1 : Set trm :=
-  {trm_seq trm0 trm1}
+  {trm1}
 def lang_set2 : Set trm :=
-  {trm_seq trm0 trm2}
+  {trm2}
 
 lemma pay_index_union_univ :
   pay_index1 ∪ pay_index2 = pay_index'
@@ -173,10 +195,15 @@ lemma pay_index_union_univ :
 lemma lang_index_union_univ :
   lang_set2 ∪ lang_set1 = lang_index'
   := by
-  unfold lang_set1 lang_set2 lang_index'
-  unfold lang_list_index' cfg_expand squeeze_trm
+  unfold lang_set1 lang_set2
+  rw [lang_index'_unfold]
   simp
-  sorry
+
+def inLang1 (a : (trm × payload)ˡ) : Prop :=
+    a.lab = 1 ∧ a.val.1 ∈ lang_set1
+
+def inLang2 (a : (trm × payload)ˡ) : Prop :=
+    a.lab = 1 ∧ a.val.1 ∈ lang_set2
 
 set_option maxRecDepth 2000 in
 set_option maxHeartbeats 6400000 in
@@ -185,7 +212,7 @@ lemma example4_spec (xv : ℤ):
     xl ~⟨i in {⟨0,p⟩ | p ∈ pay_index} ∪ {⟨1,l⟩ | l ∈ lang_index}⟩~> xv
   }
   [0| p in pay_index => prog_c1(⸨xl: Loc⸩, ⟨p.val.2⟩)]
-  [1| l in lang_index => ⟦l.val.1⟧]
+  [1| l in lang_index => l.val.fst(⸨xl: Loc⸩)]
   { v,
     fun h => ∀ l ∈ lang_index, ∃ p ∈ pay_index , h ⟨1, l⟩= h ⟨0, p⟩
   }
@@ -200,7 +227,7 @@ lemma example4_spec (xv : ℤ):
     apply disjoint_iff.mpr; simp
     apply pair_set_union_index_right
     unfold pay_index1 pay_index2; aesop
-    unfold trm1 trm2; aesop
+    unfold trm1 trm2 trm_funs; aesop
   }
   {
     conv_rhs =>  rw [Set.union_right_comm, ←Set.union_assoc]
@@ -222,7 +249,7 @@ lemma example4_spec (xv : ℤ):
   · simp; apply disjoint_label_set.mpr; simp
   · apply pair_set_union_left
     unfold lang_set1 lang_set2
-    unfold trm1 trm2; simp
+    unfold trm1 trm2 trm_funs; simp
   · unfold lang_index
     rw [lang_index'_unfold]
     apply pair_set_union_eq_right
@@ -253,6 +280,7 @@ lemma example4_spec (xv : ℤ):
      }
     apply weird_payload_index_lemma (pr := (default_trm, 10)) =>//
     { apply disjoint_label_set.mpr; aesop}
+    /- first 1/4 -/
     { unfold pay_index1 pay_index';
       simp
       dsimp [LGTM.wp, LGTM.SHTs.htrm]
@@ -312,190 +340,339 @@ lemma example4_spec (xv : ℤ):
       simp [ain] at pre
       rw [pre]
     }
+    /- second 1/4 -/
     { rw [unsimp_singleton_set]
       rw [← weird_fix_lang (p := default_payload)]
       rw [← weird_fix_payload1 (pv := 10)]
+
       unfold lang_set1
-      -- unfold bighstar bighstarDef
-      -- have qframe : (fun (x : hval (trm × payload)ˡ) ( h : hheap (trm × payload)ˡ) => h ⟨1, (trm0.trm_seq trm1, default_payload)⟩ = h ⟨0, (default_trm, 10)⟩) ===>
-      --   fun v: hval  (trm × payload)ˡ =>
-      --   (fun h =>
-      --     ∀ (a : (trm × payload)ˡ),
-      --       if a ∈ {⟨0, (default_trm, 10)⟩} then
-      --         h ⟨1, (trm0.trm_seq trm1, default_payload)⟩ = h ⟨0, (default_trm, 10)⟩
-      --       else h a = hEmpty a)
-      --  := by sorry
-      -- dsimp [LGTM.wp, LGTM.SHTs.htrm]
       unfold default_payload; simp
-      -- have eq : [∗i in ({⟨1, (trm0.trm_seq trm1, 0)⟩, ⟨0, (default_trm, 10)⟩} : Set (trm × payload)ˡ) | xl ~~> xv] = [∗i in {⟨1, (trm0.trm_seq trm1, 0)⟩}| xl ~~> xv] ∗ [∗i in {⟨0, (default_trm, 10)⟩}| xl ~~> xv] := by
-      --   unfold bighstar bighstarDef HStar.hStar instHStarHhProp hhstar
-      --     sorry
-      -- rw [eq]
-      -- have eq : {⟨0, (default_trm, 10)⟩, ⟨1, (trm0.trm_seq trm1, 0)⟩} = (⟪0, {(default_trm, 10)}⟫ ∪ ⟪1, {(trm0.trm_seq trm1, 0)}⟫) := by
-      --   unfold labSet; simp; aesop
-      -- have eq : xl ~⟨x in ⟪0, ({(default_trm, 10)} : Set (trm × payload)) ⟫⟩~> xv ∗ xl ~⟨x in ⟪1, ({(trm0.trm_seq trm1, 0)} : Set (trm × payload))⟫⟩~> xv =
-      --   xl ~⟨x in ⟪0, ({(default_trm, 10), (trm0.trm_seq trm1, 0)} : Set (trm × payload)) ⟫⟩~> xv := by
-      --   unfold hhsingle
-      yin 0: ywp; ylet; simp [subst, subst.go];
-      apply htriple_conseq; apply htriple_get (v := fun _ => xv) ; -- wrong
-      stop
-      apply htriple_get (v := fun _ => xv);
-      apply htriple_frame
-
-      erw [yfocus_lemma 0]
-      on_goal 2=> simp; apply disjoint_label_set.mpr; simp
-      dsimp
-      ystep; ysimp
-
-      stop
-      apply ywp_lemma_funs=>//
-      intro _; simp;
-      stop
-      apply hwp_of_hwpgen
-      -- yin 1: ywp;
+      yin 0: ywp; ylet; simp [subst, subst.go]
+      rw [← Set.union_singleton, ← bighstar_hhstar_disj]
+      on_goal 2=> simp
+      repeat rw [← hhsingle.eq_1]
+      apply htriple_conseq_frame (H₂ := xl ~⟨i in {⟨1, (trm1, 0)⟩}⟩~> xv); apply htriple_get (v := fun _ => xv) ;
+      { ysimp; rw [labSet]; simp }
+      ysimp
+      simp only [OfNat.ofNat, Int.ofNat]; simp
+      ywp; ylet; simp [subst, subst.go];
+      apply htriple_conseq_frame ; apply htriple_gt ; ysimp
+      ysimp; simp only [OfNat.ofNat, Zero.zero, Int.ofNat]; simp
+      ywp; yif
+      on_goal 2=> intro a ; contradiction
+      intro _;
       ystep
+      apply htriple_conseq_frame (H₂ := xl ~⟨i in {⟨1, (trm1, 0)⟩}⟩~> xv) ; apply htriple_set (hv := fun _ => xv) ; ysimp
+      ysimp
+
+      dsimp [LGTM.wp, LGTM.SHTs.htrm]
+      rw [hwp_ht_eq (ht₂ := (fun (p : (trm × payload)ˡ) => [lang| fun ⸨xk: Loc⸩ => let xx := !xk in let temp0 := xx + 1 in xk := temp0].trm_call [xl]))]
+      on_goal 2=> unfold trm1; simp [Set.EqOn, fun_insert, Set.union_empty];
+      apply ywp_lemma_funs (tfunc := fun _ => trm1) (ts := fun (p : (trm × payload)ˡ) => [xl])
+      intro _ ; rfl ; intro _ ; rfl ; intros ; rfl ; intros ; simp [get_vars, type_match]
+      simp  [Unary.func_call_ctx_prepare]
+      all_goals
+        try simp [isubstE, Unary.reduce_call_isubst]; --(try simp [Unary.isubst, Unary.isubst.go])--; (srw ?Unary.guard_pos; all_goals try rfl)
+        try simp [wpgen]
+        -- try simp [substE, Unary.reduce_call_subst]; (srw ?Unary.subst ?Unary.subst.go ?Unary.subst /==/- ?Unary.guard_pos; all_goals try rfl-/)
+        -- try simp [substlE, Unary.reduce_call_substl]; (srw ?Unary.substl ?Unary.substl.go ?Unary.substl /==/- ?Unary.guard_pos; all_goals try rfl-/)
+        try simp [AList.lookup, List.mkAlist, List.eraseP, List.dlookup]
+      ywp; ylet; simp [subst, subst.go]
+      rw [hhstar_comm]
+      apply htriple_conseq_frame (H₂ := xl ~⟨a in {⟨0, (default_trm, 10)⟩}⟩~> val_int (xv + 1 )); apply htriple_get (v := fun _ => xv);
+      { repeat rw [labSet]; simp; rw [labSet]; simp }
+      ysimp
+      ystep
+      apply htriple_conseq_frame (H₂ := xl ~⟨a in {⟨0, (default_trm, 10)⟩}⟩~> val_int (xv + 1 )); apply htriple_set (hv := fun _ => xv);
+      { ysimp; rw [labSet]; simp }
+      ysimp
+      rw [bighstar_hhstar_disj, Set.union_singleton]
+      on_goal 2=> rw [labSet]; simp
+      rw [labSet]; simp
+
+      unfold hhimpl
+      unfold bighstar bighstarDef
+      simp;
+      intro hh hl
+      have hl1 := hl ⟨1, (trm1, 0)⟩
+      have hl2 := hl ⟨0, (default_trm, 10)⟩
+      simp_all
+      rw [hl1, hl2]
     }
-  · dsimp
-    unfold lang_set2
-    have eq :
-      (fun hv' =>
-      hhstar (fun h : hheap (trm × payload)ˡ =>  ∀ ll ∈ lang_set1, ∃ pp ∈ pay_index1,  h ⟨1, (ll,0)⟩ = h ⟨0, (default_trm,pp) ⟩)
-      (fun h : hheap (trm × payload)ˡ =>  ∀ ll ∈ lang_set2, ∃ pp ∈ pay_index2,  h ⟨1, (ll,0)⟩ = h ⟨0, (default_trm,pp) ⟩) )
-       ===>
-       (fun hv' h : hheap (trm × payload)ˡ => ∀ ll ∈ lang_index, ∃ pp ∈ pay_index, h ⟨1, ll⟩ = h ⟨0, pp⟩):= by
-      sorry
-    stop
-    apply htriple_conseq
-    rw [eq]
-    /- Step 2: Lang -/
-    apply weird_lang_lemma=>//
-    { apply disjoint_label_set.mpr; aesop}
-    /- Step 3: Payload -/
-    rw [← bighstar_hhstar_disj_dir (s₁ := {⟨0,(default_trm,p)⟩ | p ∈ pay_index1 \ {10}}) (s₂ := {⟨0,(default_trm,10)⟩} ∪ {⟨ 1, (l,default_payload)⟩ | l ∈ lang_set1} )]
+  /- Right Part -/
+  · unfold lang_set2
+    set H₃ := (fun h : hheap (trm × payload)ˡ =>
+        ∀ ll ∈ {x | ∃ l ∈ lang_set1, (l, default_payload) = x},
+        ∃ pp ∈ {x | ∃ p ∈ pay_index1, (default_trm, p) = x}, h ⟨1, ll⟩ = h ⟨0, pp⟩) with hH3
+    set H₄ := [∗i in ({x | ∃ p ∈ pay_index2, ⟨0, (default_trm, p)⟩ = x} : Set (trm × payload)ˡ) ∪ ({x | ∃ l ∈ ({trm2}: Set trm), ⟨1, (l, default_payload)⟩ = x} : Set (trm × payload)ˡ)| (fun i ↦ xl) i ~~> (fun i ↦ xv) i] with hH4
+    dsimp
+    have weakenH3 : H₃ ==> fun (h : (hheap (trm × payload)ˡ))=> ∀ ll ∈ {x | ∃ l ∈ lang_set1, (l, default_payload) = x}, ∃ pp ∈ pay_index, h ⟨1, ll⟩ = h ⟨0, pp⟩ := by
+      rw [hH3]
+      intro hh
+      apply hheap_weaken_forall'
+      unfold pay_index pay_index' pay_index1 pay_index' default_trm
+      simp
+    rw [hhstar_symbol_replace]
+    have reH3 := hhimpl_frame_l H₃ (fun (h : (hheap (trm × payload)ˡ))=> ∀ ll ∈ {x | ∃ l ∈ lang_set1, (l, default_payload) = x}, ∃ pp ∈ pay_index, h ⟨1, ll⟩ = h ⟨0, pp⟩) H₄ weakenH3
+    rw [← hhstar_symbol_replace]
+    rw [← hhstar_symbol_replace] at reH3
+    apply hhimpl_trans=>//
+
+    rw [hqstar_disjoint_lang_index_eq (lang_set1 := lang_set1) (lang_set2:=lang_set2) (lang_index := lang_index) (pay_index := pay_index) (default_payload := default_payload)]
     rotate_left
-    { apply disjoint_iff.mpr
-      unfold lang_set1
-      aesop }
+    { unfold lang_index
+      rw [←lang_index_union_univ]
+      unfold lang_set1 lang_set2 default_payload
+      aesop
+    }
     {
-      unfold pay_index1 pay_index' lang_set1; simp
-      apply congr_arg
-      ext x
-      constructor
-      · rintro ⟨p, hp_pos, rfl⟩
-        by_cases h10 : p = 10=>//
-      · rintro (rfl | ⟨p, ⟨hp_pos, hp_ne⟩, rfl⟩)=>//
-     }
-    apply weird_payload_index_lemma (pr := (default_trm, 10)) =>//
+      unfold lang_set1 lang_set2
+      unfold trm1 trm2 trm_funs
+      simp
+    }
+    rw [hqstar_symbol_replace]
+    have wpfram := LGTM.wp_frame (sht := [{ s := ⟪0, {x | ∃ p ∈ pay_index2, (default_trm, p) = x}⟫, ht := fun p ↦ prog_c1.trm_call [xl, [lang| ⟨p.val.2⟩]] },
+      { s := ⟪1, {x | ∃ l ∈ ({trm2}:Set trm), (l, default_payload) = x}⟫, ht := fun l ↦ l.val.1.trm_call [xl] }]) ((fun hv' (h:hheap (trm × payload)ˡ) => ∀ ll ∈ {x | ∃ l ∈ lang_set2, (l, default_payload) = x}, ∃ pp ∈ pay_index, h ⟨1, ll⟩ = h ⟨0, pp⟩))
+      (fun h ↦ ∀ ll ∈ {x | ∃ l ∈ lang_set1, (l, default_payload) = x}, ∃ pp ∈ pay_index, h ⟨1, ll⟩ = h ⟨0, pp⟩)
+    apply hhimpl_trans_r=>//
+    rw [hhstar_comm (hH₂ := H₄)]
+    apply hhimpl_frame_l
+    rw [hH4]
+    clear wpfram reH3 hH4 weakenH3 hH3 H₃ H₄
+
+    rw [unsimp_singleton_set]
+    rw [← weird_fix_lang (p := default_payload)]
+    rw [← bighstar_hhstar_disj]
+    rw [← bighstar_hhstar_disj_dir (s₁ := {x | ∃ p ∈ pay_index2 \ {-10}, ⟨0, (default_trm, p)⟩ = x}) (s₂ := {⟨0, (default_trm, -10)⟩})]=>//
+    rotate_left
+    have eq: ( {⟨0, (default_trm, -10)⟩} : Set (trm × payload)ˡ )= ({ x | ∃ p ∈ ({-10} : Set payload), ⟨0, (default_trm, p)⟩ = x} : Set (trm × payload)ˡ):= by simp
+    rw [eq]; clear eq
+    rw [pair_set_union_index_eq_left]; simp; unfold pay_index2 pay_index'; simp
+
+    rw [hhstar_assoc]
+    apply weird_payload_index_lemma2
+      (pr := (default_trm, -10))
+      (s₁ := {x | ∃ p ∈ pay_index2, (default_trm, p) = x})
+      (H₁ := [∗i in {x | ∃ p ∈ pay_index2 \ {-10}, ⟨0, (default_trm, p)⟩ = x}| xl ~~> xv])=>//
+    { apply disjoint_label_set.mpr; simp}
+    { unfold pay_index; simp; unfold pay_index2; simp }
+    /- Third 1/4 -/
+    { unfold pay_index2 pay_index';
+      simp
+      dsimp [LGTM.wp, LGTM.SHTs.htrm]
+      rw [hwp_ht_eq (ht₂ := (fun (p : (trm × payload)ˡ) => prog_c1.trm_call [xl, [lang| ⟨p.val.2⟩]]))] --remove union set
+      on_goal 2=> simp only [Set.EqOn, fun_insert, Set.union_empty] ; intro a b ; simp only [b, reduceIte]
+      unfold prog_c1 --; yapp
+      apply ywp_lemma_funs (tfunc := fun _ => prog_c1) (ts := fun (p : (trm × payload)ˡ) => [xl, [lang| ⟨p.val.2⟩]])
+      intro _ ; rfl ; intro _ ; rfl ; intros ; rfl ; intros ; simp [get_vars, type_match]
+      -- unfold prog_c1
+      simp  [Unary.func_call_ctx_prepare]
+      all_goals
+        try simp [isubstE, Unary.reduce_call_isubst]; --(try simp [Unary.isubst, Unary.isubst.go])--; (srw ?Unary.guard_pos; all_goals try rfl)
+        try simp [wpgen]
+        try simp [AList.lookup, List.mkAlist, List.eraseP, List.dlookup]
+      apply hwp_of_hwpgen
+      simp [subst, subst.go]
+      ylet
+      have eq : ({x | ∃ (p : payload), (p ≤ 0 ∧ ¬p = -10) ∧ ⟨0, (default_trm, p)⟩ = x} : Set (trm × payload)ˡ)
+        = (⟪0, {x | ∃ p, p ≤ 0 ∧ (default_trm, p) = x} \ {(default_trm, -10)}⟫ : Set (trm × payload)ˡ)
+        := by
+        ext a ; rcases a with ⟨l, ⟨a, b⟩⟩ ; simp ; aesop
+          -- ext
+      rw [eq] ; clear eq --; yapp htriple_get
+      apply htriple_conseq ; apply htriple_get (v := fun _ => xv) ; apply hhimpl_refl
+      ysimp
+      ywp ; ylet
+      apply htriple_conseq_frame ; apply htriple_gt ; ysimp
+      ysimp ; simp [subst, subst.go]
+
+      rw [hwp_ht_eq (ht₂ := (fun a ↦
+      [lang|
+        if false then
+          let temp1 := xv + 1 in
+          xl := temp1
+        else
+          let temp2 := xv + 2 in
+          xl := temp2]))]
+      on_goal 2=> simp only [Set.EqOn, fun_insert, Set.union_empty] ; rintro ⟨l, ⟨a , b⟩⟩ bb ; congr ; simp at bb ⊢ ; aesop
+      ywp ; yif
+      on_goal 1=> intro a ; contradiction
+      intro _
+      ystep
+      apply htriple_conseq ; apply htriple_set (hv := fun _ => xv) ; apply hhimpl_refl
+      ysimp
+      unfold hhsingle bighstar bighstarDef hsingle hhimpl
+      simp
+      intro ha pre aa hlab --hpay hgt0 heq hvalnot
+      specialize pre aa
+      have ain : ¬ aa ∈ ⟪0, {x | ∃ p, p ≤ 0 ∧ (default_trm, p) = x} \ {(default_trm, -10)}⟫ := by
+        simp;
+        intro h_in hx hgt hheq
+        have := hlab h_in hx hgt hheq
+        exact this
+      simp [ain] at pre
+      rw [pre]
+    }
+    /- Final 1/4 -/
+    dsimp
+    rw [← weird_fix_payload1 (pv := -10)]
+    unfold default_payload; simp
+    yin 0: ywp; ylet; simp [subst, subst.go]
+    -- rw [← hhstar_symbol_replace (hH₁ := [∗i in {⟨1, (trm2, 0)⟩}| xl ~~> xv]) (hH₂ := H₃)]
+    -- apply htriple_conseq_frame (H₂ := hhstar [∗i in {⟨1, (trm2, 0)⟩}| xl ~~> xv] H₃); apply htriple_get (v := fun _ => xv) ;
+    apply htriple_conseq_frame (H₂ := [∗i in {⟨1, (trm2, 0)⟩}| xl ~~> xv]); apply htriple_get (v := fun _ => xv) ;
+    { ysimp; rw [labSet]; simp }
+    ysimp
+    simp only [OfNat.ofNat, Int.ofNat]; simp
+    ywp; ylet; simp [subst, subst.go];
+    apply htriple_conseq_frame ; apply htriple_gt ; ysimp
+    ysimp; simp only [OfNat.ofNat, Zero.zero, Int.ofNat]; simp
+    ywp; yif
+    on_goal 1=> intro a ; contradiction
+    intro _;
+    ystep
+    apply htriple_conseq_frame (H₂ := [∗i in {⟨1, (trm2, 0)⟩}| xl ~~> xv]) ; apply htriple_set (hv := fun _ => xv) ; ysimp
+    ysimp
+
+    dsimp [LGTM.wp, LGTM.SHTs.htrm]
+    rw [hwp_ht_eq (ht₂ := (fun (p : (trm × payload)ˡ) => [lang| fun ⸨xr: Loc⸩ => let xx := !xr in let temp0 := xx + 2 in xr := temp0].trm_call [xl]))]
+    on_goal 2=> unfold trm2; simp [Set.EqOn, fun_insert, Set.union_empty];
+    apply ywp_lemma_funs (tfunc := fun _ => trm2) (ts := fun (p : (trm × payload)ˡ) => [xl])
+    intro _ ; unfold trm2 trm_funs; simp ;
+    intro _ ; rfl ; intros ; rfl ; intros ; simp [get_vars, type_match]
+    simp  [Unary.func_call_ctx_prepare]
+    all_goals
+      try simp [isubstE, Unary.reduce_call_isubst]; --(try simp [Unary.isubst, Unary.isubst.go])--; (srw ?Unary.guard_pos; all_goals try rfl)
+      try simp [wpgen]
+      try simp [AList.lookup, List.mkAlist, List.eraseP, List.dlookup]
+    ywp; ylet; simp [subst, subst.go]
+    rw [hhstar_comm]
+    -- rw [hhstar_symbol_replace (hH₁ := [∗i in {⟨1, (trm2, 0)⟩}| xl ~~> xv]) (hH₂ := H₃)]
+    -- rw [hhstar_assoc]
+    -- rw [← hhstar_symbol_replace (hH₁ := H₃)]
+    have eq : (xl ~⟨a in ⟪OfNat.ofNat (OfNat.ofNat (OfNat.ofNat 0)), {(default_trm, -10)}⟫⟩~> val_int (xv + 2)) = (xl ~⟨a in ⟪0, {(default_trm, -10)}⟫⟩~> val_int (xv + 2)) := by
+      simp
+    rw [eq]; clear eq
+    apply htriple_conseq_frame (H₂ := [∗i in {⟨0, (default_trm, -10)⟩}| xl ~~> val_int (xv + 2)]); apply htriple_get (v := fun _ => xv);
+    { repeat rw [labSet]; simp; rw [labSet]; unfold hhsingle; simp; }
+    ysimp
+    ystep
+    apply htriple_conseq_frame (H₂ := [∗i in {⟨0, (default_trm, -10)⟩}| xl ~~> val_int (xv + 2)]); apply htriple_set (hv := fun _ => xv);
+    { ysimp}
+    ysimp
+
+    rw [bighstar_hhstar_disj, Set.union_singleton]
+    on_goal 2=> rw [labSet]; simp
+    rw [labSet]; simp
+    unfold lang_set2; simp
+    unfold hhimpl
+    unfold bighstar bighstarDef
+    simp;
+    intro hh hl
+    have hl1 := hl ⟨1, (trm2, 0)⟩
+    have hl2 := hl ⟨0, (default_trm, -10)⟩
+    simp_all
+    rw [hl1, hl2]
 
 #check Function.partialInv_left
 #print bighstar_hhstar_disj
--- #check ystep
 
-lemma hharray_disj (s₁ : Set α) (f : ℤ → val):
-  arr⟨s₁⟩(p , x in n =>f x) ∗ arr⟨⋆ \ s₁⟩(p , x in n =>f x) = arr⟨⋆⟩(p , x in n =>f x) :=by
-  have tmp : arr⟨⋆⟩(p , x in n =>f x) = arr⟨s₁ ∪ (⋆ \ s₁)⟩(p , x in n =>f x) := by
-    congr!
-    exact Eq.symm (Set.union_diff_cancel' (fun ⦃a⦄ a ↦ a) fun ⦃a⦄ a ↦ trivial)
-  rw [tmp]
-  unfold hharrayFun
-  apply eq_comm.mpr
-  symm
-  apply bighstar_hhstar_disj (s₂ := ⋆ \ s₁)=>//
-  exact Set.disjoint_sdiff_right
+-- lemma hharray_disj (s₁ : Set α) (f : ℤ → val):
+--   arr⟨s₁⟩(p , x in n =>f x) ∗ arr⟨⋆ \ s₁⟩(p , x in n =>f x) = arr⟨⋆⟩(p , x in n =>f x) :=by
+--   have tmp : arr⟨⋆⟩(p , x in n =>f x) = arr⟨s₁ ∪ (⋆ \ s₁)⟩(p , x in n =>f x) := by
+--     congr!
+--     exact Eq.symm (Set.union_diff_cancel' (fun ⦃a⦄ a ↦ a) fun ⦃a⦄ a ↦ trivial)
+--   rw [tmp]
+--   unfold hharrayFun
+--   apply eq_comm.mpr
+--   symm
+--   apply bighstar_hhstar_disj (s₂ := ⋆ \ s₁)=>//
+--   exact Set.disjoint_sdiff_right
 
-def left_lang_index : Set (trm ⊕ payload):= {l:trm ⊕ payload |
-      match l with
-      | Sum.inl t => t = [lang| x := x + 1] ∧ cfg1.Generates (expand_trm t)
-      | Sum.inr _ => False}
+-- lemma example4_spec_hete (f : ℤ -> val):
+--   {
+--     -- ⊤
+--     -- [∗ in Set.univ | H ] ∗
+--     arr⟨⋆⟩(xptr , i in 1 =>f i) -- replace it
+--   }
+--   [0| Sum.inr| p in pay_index' => prog_c1(⟨f 1⟩, ⟨p.val⟩)]
+--   [1| Sum.inl| l in lang_index' => ⟦l.val⟧]
 
-def right_lang_index : Set (trm ⊕ payload):= {l:trm ⊕ payload |
-      match l with
-      | Sum.inl t => t = [lang| x := x + 2] ∧ cfg1.Generates (expand_trm t)
-      | Sum.inr _ => False}
+--   { v,
+--     fun h => ∀ ll ∈ lang_index', ∃ pp , pp ∈ pay_index' ∧ h ⟨1, Sum.inl ll⟩ = h ⟨0, Sum.inr pp⟩
+--   } := by
+--   unfold LGTM.triple
+--   unfold LGTM.HSHT.mkSHT LGTM.Labeled.map Set.image
+--   dsimp
+--   stop
+--   apply weird_grmdisj_lemma
+--     (s' := left_lang_index)
+--     (H := arr⟨⟪0,⋆ ⟫⟩(xptr , i in 1 =>f i))
+--     (H₁ := arr⟨⟪1,left_lang_index⟫⟩(xptr , i in 1 =>f i))
+--     (H₂ := arr⟨⟪1,right_lang_index⟫⟩(xptr , i in 1 =>f i))
+--     (HH := arr⟨⋆⟩(xptr , i in 1 =>f i))
+--     =>//
+--   · unfold labSet pay_index; simp_all
+--   · unfold labSet lang_index lang_index'; simp_all
+--   · unfold left_lang_index lang_index
+--     simp_all
+--   · sorry
+--   · sorry
+--   · sorry
+--   /- left part: goes to false branch-/
+--   · set pay_s := { p | p<=0 ∧ p ∈ pay_index'}
+--     set pay_s' : Set (trm ⊕ payload) := (fun p => Sum.inr p) '' pay_s
+--     set hsub := pay_index' \ pay_s
+--     set hsub_sum : Set (trm ⊕ payload)ˡ := (fun p => ⟨0, Sum.inr p⟩) '' hsub
+--     set H₁ := arr⟨hsub_sum⟩(xptr , i in 1 =>f i)
+--     set H₂ := arr⟨⋆ \ hsub_sum⟩(xptr , i in 1 =>f i)
+--     have trans_pre : H₁ ∗ H₂ = arr⟨⋆⟩(xptr , i in 1 =>f i) := by
+--       unfold H₁ H₂
+--       apply hharray_disj (s₁ := hsub_sum)
+--       aesop
+--     rw [← trans_pre]
+--     apply weird_weaken_lemma (s := pay_index) (s'' := lang_index \ {(Sum.inl [lang| x := x + 1])}) (s' := pay_s') (H₁ := H₁) (H₂ := H₂) =>//
+--     · unfold labSet pay_index; simp_all
+--     · unfold pay_index pay_s'
+--       aesop
+--     · simp_all
+--       apply Set.disjoint_iff_inter_eq_empty.mpr
+--       aesop
+--     /- left part: solvable using ystep and yif if can do case analysis inside ht -/
+--     · simp_all; unfold H₁ hsub_sum
+--       apply ysubst_lemma («σ» := Sum.getRight!)=>//
+--       sorry
+--     /- right part: shrink payload to p<=0 -/
+--     · simp
+--       sorry
+--   /- right part: goes to true branch-/
+--   · set pay_s := { p | p>0 ∧ p ∈ pay_index'}
+--     set pay_s' : Set (trm ⊕ payload) := (fun p => Sum.inr p) '' pay_s
+--     set hsub := pay_index' \ pay_s
+--     set hsub_sum : Set (trm ⊕ payload)ˡ := (fun p => ⟨0, Sum.inr p⟩) '' hsub
+--     set H₁ := arr⟨hsub_sum⟩(xptr , i in 1 =>f i)
+--     set H₂ := arr⟨⋆ \ hsub_sum⟩(xptr , i in 1 =>f i)
+--     have trans_pre : H₁ ∗ H₂ = arr⟨⋆⟩(xptr , i in 1 =>f i) := by
+--       unfold H₁ H₂
+--       apply hharray_disj (s₁ := hsub_sum)
+--       aesop
+--     rw [← trans_pre]
+--     apply weird_weaken_lemma (s := pay_index) (s'' := {(Sum.inl [lang| x := x + 1])}) (s' := pay_s') (H₁ := H₁) (H₂ := H₂) =>//
+--     · unfold labSet pay_index; simp_all
+--     · unfold pay_index pay_s'
+--       simp_all
+--     · simp_all
+--       apply Set.disjoint_iff_inter_eq_empty.mpr
+--       aesop
+--     /- left part: solvable using ystep and yif if can do case analysis inside ht-/
+--     · unfold H₁ LGTM.wp prog_c1
+--       simp_all
+--       -- cases hpi : Function.partialInv (fun x : payloadˡ => ⟨x.lab, Sum.inr x.val⟩) a
+--       apply weird_index_subst_left
+--       sorry
+--     /- right part: shrink p to p>0-/
+--     · unfold H₂
+--       sorry
 
-lemma example4_spec_hete (f : ℤ -> val):
-  {
-    -- ⊤
-    -- [∗ in Set.univ | H ] ∗
-    arr⟨⋆⟩(xptr , i in 1 =>f i) -- replace it
-  }
-  [0| Sum.inr| p in pay_index' => prog_c1(⟨f 1⟩, ⟨p.val⟩)]
-  [1| Sum.inl| l in lang_index' => ⟦l.val⟧]
-
-  { v,
-    fun h => ∀ ll ∈ lang_index', ∃ pp , pp ∈ pay_index' ∧ h ⟨1, Sum.inl ll⟩ = h ⟨0, Sum.inr pp⟩
-  } := by
-  unfold LGTM.triple
-  unfold LGTM.HSHT.mkSHT LGTM.Labeled.map Set.image
-  dsimp
-  stop
-  apply weird_grmdisj_lemma
-    (s' := left_lang_index)
-    (H := arr⟨⟪0,⋆ ⟫⟩(xptr , i in 1 =>f i))
-    (H₁ := arr⟨⟪1,left_lang_index⟫⟩(xptr , i in 1 =>f i))
-    (H₂ := arr⟨⟪1,right_lang_index⟫⟩(xptr , i in 1 =>f i))
-    (HH := arr⟨⋆⟩(xptr , i in 1 =>f i))
-    =>//
-  · unfold labSet pay_index; simp_all
-  · unfold labSet lang_index lang_index'; simp_all
-  · unfold left_lang_index lang_index
-    simp_all
-  · sorry
-  · sorry
-  · sorry
-  /- left part: goes to false branch-/
-  · set pay_s := { p | p<=0 ∧ p ∈ pay_index'}
-    set pay_s' : Set (trm ⊕ payload) := (fun p => Sum.inr p) '' pay_s
-    set hsub := pay_index' \ pay_s
-    set hsub_sum : Set (trm ⊕ payload)ˡ := (fun p => ⟨0, Sum.inr p⟩) '' hsub
-    set H₁ := arr⟨hsub_sum⟩(xptr , i in 1 =>f i)
-    set H₂ := arr⟨⋆ \ hsub_sum⟩(xptr , i in 1 =>f i)
-    have trans_pre : H₁ ∗ H₂ = arr⟨⋆⟩(xptr , i in 1 =>f i) := by
-      unfold H₁ H₂
-      apply hharray_disj (s₁ := hsub_sum)
-      aesop
-    rw [← trans_pre]
-    apply weird_weaken_lemma (s := pay_index) (s'' := lang_index \ {(Sum.inl [lang| x := x + 1])}) (s' := pay_s') (H₁ := H₁) (H₂ := H₂) =>//
-    · unfold labSet pay_index; simp_all
-    · unfold pay_index pay_s'
-      aesop
-    · simp_all
-      apply Set.disjoint_iff_inter_eq_empty.mpr
-      aesop
-    /- left part: solvable using ystep and yif if can do case analysis inside ht -/
-    · simp_all; unfold H₁ hsub_sum
-      apply ysubst_lemma («σ» := Sum.getRight!)=>//
-      sorry
-    /- right part: shrink payload to p<=0 -/
-    · simp
-      sorry
-  /- right part: goes to true branch-/
-  · set pay_s := { p | p>0 ∧ p ∈ pay_index'}
-    set pay_s' : Set (trm ⊕ payload) := (fun p => Sum.inr p) '' pay_s
-    set hsub := pay_index' \ pay_s
-    set hsub_sum : Set (trm ⊕ payload)ˡ := (fun p => ⟨0, Sum.inr p⟩) '' hsub
-    set H₁ := arr⟨hsub_sum⟩(xptr , i in 1 =>f i)
-    set H₂ := arr⟨⋆ \ hsub_sum⟩(xptr , i in 1 =>f i)
-    have trans_pre : H₁ ∗ H₂ = arr⟨⋆⟩(xptr , i in 1 =>f i) := by
-      unfold H₁ H₂
-      apply hharray_disj (s₁ := hsub_sum)
-      aesop
-    rw [← trans_pre]
-    apply weird_weaken_lemma (s := pay_index) (s'' := {(Sum.inl [lang| x := x + 1])}) (s' := pay_s') (H₁ := H₁) (H₂ := H₂) =>//
-    · unfold labSet pay_index; simp_all
-    · unfold pay_index pay_s'
-      simp_all
-    · simp_all
-      apply Set.disjoint_iff_inter_eq_empty.mpr
-      aesop
-    /- left part: solvable using ystep and yif if can do case analysis inside ht-/
-    · unfold H₁ LGTM.wp prog_c1
-      simp_all
-      -- cases hpi : Function.partialInv (fun x : payloadˡ => ⟨x.lab, Sum.inr x.val⟩) a
-      apply weird_index_subst_left
-      sorry
-    /- right part: shrink p to p>0-/
-    · unfold H₂
-      sorry
 
 end WeirdLogic
